platform/facade/CompileUnit.v
@@ -1,0 +1,31 @@
+Set Implicit Arguments.
+
+Require Import DFacade DFModule.
+Require Import StringMap WordMap GLabelMap.
+
+Notation module_name := "dfmodule".
+Notation fun_name := "dffun".
+Notation argvar1 := "arg1".
+Notation argvar2 := "arg2".
+Notation argvars := (argvar1 :: argvar2 :: nil).
+Notation retvar := "ret".
+
+Record CompileUnit (ADTValue : Type) := 
+  {
+    prog : Stmt;
+    no_assign_to_args : is_disjoint (assigned prog) (StringSetFacts.of_list argvars) = true;
+    syntax_ok : is_syntax_ok prog = true;
+    compile_syntax_ok : FModule.is_syntax_ok (CompileDFacade.compile_op (Build_OperationalSpec argvars retvar prog eq_refl eq_refl no_assign_to_args eq_refl eq_refl syntax_ok)) = true;
+    imports : GLabelMap.t (AxiomaticSpec ADTValue);
+    pre_cond : Value ADTValue -> Value ADTValue -> Prop;
+    post_cond : Value ADTValue -> Value ADTValue -> Value ADTValue -> Prop;
+    pre_safe : forall st value1 value2, 
+                 StringMap.Equal st (StringMapFacts.make_map (argvar1 :: argvar2 :: nil) (value1 :: value2 :: nil)) -> 
+                 pre_cond value1 value2 -> 
+                 DFacade.Safe (GLabelMap.map (@Axiomatic _) imports) prog st;
+    pre_runsto_post : forall st st' value1 value2, 
+                        StringMap.Equal st (StringMapFacts.make_map (argvar1 :: argvar2 :: nil) (value1 :: value2 :: nil)) -> 
+                        pre_cond value1 value2 -> DFacade.RunsTo (GLabelMap.map (@Axiomatic _) imports) prog st st' -> 
+                        exists ret, StringMap.Equal st' (StringMapFacts.make_map (retvar :: nil) (ret :: nil)) /\ post_cond value1 value2 ret
+  }.
+
